admitted timeseries interaction with msv

src/program_proof/pav/core.v
@@ -7,21 +7,25 @@ Notation uid_ty := w64 (only parsing).
 Notation ver_ty := nat (only parsing).
 Notation epoch_ty := nat (only parsing).
 Notation pk_ty := (list w8) (only parsing).
-Notation map_ty := (gmap (uid_ty * ver_ty) pk_ty) (only parsing).
+Notation map_label_ty := (uid_ty * ver_ty)%type (only parsing).
+Notation map_val_ty := (epoch_ty * pk_ty)%type (only parsing).
+Notation map_ty := (gmap map_label_ty map_val_ty) (only parsing).
 (* sub-maps are useful for helping us state non-existence of
-certain keys in a way that they carry across map subsets. *)
-Notation submap_ty := (gmap (uid_ty * ver_ty) (option pk_ty)) (only parsing).
+keys in a way that they carry across map subsets. *)
+Notation submap_ty := (gmap map_label_ty (option map_val_ty)) (only parsing).
 
 Section msv.
 
-Definition msv_aux (m : map_ty) uid pks :=
-  (∀ i, i < length pks → m !! (uid, i) = pks !! i).
-
 (* maximum sequence of versions. *)
-Definition msv m uid pks :=
-  msv_aux m uid pks ∧
-  m !! (uid, (length pks)) = None.
 
+Definition msv_aux (m : map_ty) uid vals :=
+  (∀ i, i < length vals → m !! (uid, i) = vals !! i).
+
+Definition msv m uid vals :=
+  msv_aux m uid vals ∧
+  m !! (uid, (length vals)) = None.
+
+(* TODO: upstream. *)
 Lemma lookup_snoc {A} (l : list A) (x : A) :
   (l ++ [x]) !! (length l) = Some x.
 Proof. by opose proof (proj2 (lookup_snoc_Some x l (length l) x) _) as H; [naive_solver|]. Qed.
@@ -37,14 +41,14 @@ Proof.
     by rewrite lookup_snoc in HM.
 Qed.
 
-Lemma msv_aux_agree {m uid pks0 pks1} :
-  msv_aux m uid pks0 →
-  msv_aux m uid pks1 →
-  length pks0 = length pks1 →
-  pks0 = pks1.
+Lemma msv_aux_agree {m uid vals0 vals1} :
+  msv_aux m uid vals0 →
+  msv_aux m uid vals1 →
+  length vals0 = length vals1 →
+  vals0 = vals1.
 Proof.
-  revert pks1. induction pks0 as [|x0 l0 IH] using rev_ind;
-    destruct pks1 as [|x1 l1 _] using rev_ind.
+  revert vals1. induction vals0 as [|x0 l0 IH] using rev_ind;
+    destruct vals1 as [|x1 l1 _] using rev_ind.
   - done.
   - rewrite length_app/=. lia.
   - rewrite length_app/=. lia.
@@ -54,34 +58,34 @@ Proof.
     simplify_map_eq/=. ospecialize (IH l1 _ _ _); [done..|lia|]. naive_solver.
 Qed.
 
-Lemma msv_len_agree_aux {m uid pks0 pks1} :
-  msv m uid pks0 →
-  msv m uid pks1 →
-  length pks0 < length pks1 →
+Lemma msv_len_agree_aux {m uid vals0 vals1} :
+  msv m uid vals0 →
+  msv m uid vals1 →
+  length vals0 < length vals1 →
   False.
 Proof.
   intros HM0 HM1 ?. destruct HM0 as [_ HM0]. destruct HM1 as [HM1 _].
-  ospecialize (HM1 (length pks0) _); [lia|].
-  opose proof (lookup_lt_is_Some_2 pks1 (length pks0) _) as [? Hsome]; [lia|].
+  ospecialize (HM1 (length vals0) _); [lia|].
+  opose proof (lookup_lt_is_Some_2 vals1 (length vals0) _) as [? Hsome]; [lia|].
   rewrite Hsome in HM1. naive_solver.
 Qed.
 
-Lemma msv_len_agree {m uid pks0 pks1} :
-  msv m uid pks0 →
-  msv m uid pks1 →
-  length pks0 = length pks1.
+Lemma msv_len_agree {m uid vals0 vals1} :
+  msv m uid vals0 →
+  msv m uid vals1 →
+  length vals0 = length vals1.
 Proof.
   intros ??.
-  destruct (decide (length pks0 = length pks1)) as [?|?]; [done|].
-  exfalso. destruct (decide (length pks0 < length pks1)) as [?|?].
-  - eapply (msv_len_agree_aux (pks0:=pks0) (pks1:=pks1)); [done..|lia].
-  - eapply (msv_len_agree_aux (pks0:=pks1) (pks1:=pks0)); [done..|lia].
+  destruct (decide (length vals0 = length vals1)) as [?|?]; [done|].
+  exfalso. destruct (decide (length vals0 < length vals1)) as [?|?].
+  - eapply (msv_len_agree_aux (vals0:=vals0) (vals1:=vals1)); [done..|lia].
+  - eapply (msv_len_agree_aux (vals0:=vals1) (vals1:=vals0)); [done..|lia].
 Qed.
 
-Lemma msv_agree {m uid pks0 pks1} :
-  msv m uid pks0 →
-  msv m uid pks1 →
-  pks0 = pks1.
+Lemma msv_agree {m uid vals0 vals1} :
+  msv m uid vals0 →
+  msv m uid vals1 →
+  vals0 = vals1.
 Proof.
   intros HM0 HM1. eapply msv_aux_agree.
   - by destruct HM0 as [? _].
@@ -90,3 +94,74 @@ Proof.
 Qed.
 
 End msv.
+
+Section ts_msv.
+
+(* timeseries and its interaction with msv. *)
+
+Definition maps_mono (ms : list map_ty) :=
+  ∀ i j mi mj,
+  ms !! i = Some mi →
+  ms !! j = Some mj →
+  i ≤ j →
+  mi ⊆ mj.
+
+(* note: auditor allows entry to be added after expected.
+but originating client ensures that doesn't happen. *)
+Definition maps_epoch_ok (ms : list map_ty) :=
+  ∀ ep m_ep (k : uid_ty * ver_ty) ep' (pk : pk_ty),
+  ms !! ep = Some m_ep →
+  m_ep !! k = Some (ep', pk) →
+  (* can't have new entries in an old epoch. *)
+  ep' ≤ ep.
+
+Definition adtr_inv ms := maps_mono ms ∧ maps_epoch_ok ms.
+
+Record ts_ty :=
+  mk_ts {
+    entries: list (epoch_ty * pk_ty);
+    bound: epoch_ty;
+  }.
+
+(* rets Some iff ep ≤ bound. fetches all the pk's thru ep. *)
+Fixpoint ts_get (ts : ts_ty) (ep : epoch_ty) : option (list map_val_ty). Admitted.
+
+Definition ts_epoch_mono (ts : ts_ty) :=
+  ∀ i j ep_i pk_i ep_j pk_j,
+  ts.(entries) !! i = Some (ep_i, pk_i) →
+  ts.(entries) !! j = Some (ep_j, pk_j) →
+  i < j →
+  ep_i < ep_j.
+
+Definition ts_bound_ok (ts : ts_ty) :=
+  ∀ ep pk,
+  last ts.(entries) = Some (ep, pk) →
+  ep ≤ ts.(bound).
+
+Definition ts_entry_know (ts : ts_ty) (ms : list map_ty) uid :=
+  ∀ ver ep pk m,
+  ts.(entries) !! ver = Some (ep, pk) →
+  ms !! ep = Some m →
+  m !! (uid, ver) = Some (ep, pk) ∧ m !! (uid, S ver) = None.
+
+Definition ts_bound_know (ts : ts_ty) (ms : list map_ty) uid :=
+  ∀ m,
+  ms !! ts.(bound) = Some m →
+  m !! (uid, length ts.(entries)) = None.
+
+(* maintained by client. *)
+Definition ts_inv ts ms uid :=
+  ts_epoch_mono ts ∧
+  ts_bound_ok ts ∧
+  ts_entry_know ts ms uid ∧
+  ts_bound_know ts ms uid.
+
+Lemma ts_interp ts ms uid ep m vals :
+  ts_inv ts ms uid →
+  adtr_inv ms →
+  ms !! ep = Some m →
+  ts_get ts ep = Some vals →
+  msv m uid vals.
+Proof. Admitted.
+
+End ts_msv.
